all theorems proved

ContProof.v
@@ -16,6 +16,16 @@ Import Cont.
 
 Open Scope nat_scope.
 
+Lemma entails_guard : forall P P' c k,
+  entails P P' -> guard P' c k -> guard P c k.
+Proof.
+  unfold entails, guard, Assertion_denote.
+  intros.
+  specialize (H st H1).
+  specialize (H0 st H).
+  tauto.
+Qed.  
+
 Lemma consequence_valid_continuation: forall c P P' Q Q' R1 R1' R2 R2',
   entails P' P ->
   entails Q Q' ->
@@ -24,8 +34,15 @@ Lemma consequence_valid_continuation: forall c P P' Q Q' R1 R1' R2 R2',
   valid_continuation P c Q R1 R2 ->
   valid_continuation P' c Q' R1' R2'.
 Proof.
-Admitted.
-
+  unfold valid_continuation.
+  intros.
+  pose proof (entails_guard _ _ _ _ H0 H4).
+  pose proof (entails_guard _ _ _ _ H1 H5).
+  pose proof (entails_guard _ _ _ _ H2 H6).
+  specialize (H3 k H7 H8 H9).
+  pose proof (entails_guard _ _ _ _ H H3).
+  tauto.
+Qed.
 
 Lemma safe_mstep_pre: forall c k st c' k' st',
   safe c k st ->
@@ -1588,19 +1605,365 @@ Qed.
 
 (* Print Assumptions nocontinue_valid_continuation. *)
 
+Inductive if_seq_sim : (com * continuation) -> (com * continuation) -> Prop :=
+  | IS_sim_id : forall c k, if_seq_sim (c, k) (c, k)
+  | IS_sim_ifseq : forall b c1 c2 c3 k,
+  if_seq_sim (CSeq (CIf b c1 c2) c3, k) (CIf b (CSeq c1 c3) (CSeq c2 c3), k)
+  | IS_sim_seq : forall b c1 c2 c3 k,
+  if_seq_sim (CIf b c1 c2, KSeq c3 :: k) (CIf b (CSeq c1 c3) (CSeq c2 c3), k)
+  (* | IS_sim_bfalse : forall c1 c2 c3 k,
+      if_seq_sim (CIf BFalse c1 c2, KSeq c3 :: k) (CSeq c1 c3, k)
+  | IS_sim_btrue : forall c1 c2 c3 k,
+      if_seq_sim (CIf BTrue c1 c2, KSeq c3 :: k) (CSeq c2 c3, k) *)
+  .
+
+Lemma if_seq_sim_is_simulation : simulation if_seq_sim.
+Proof.
+  unfold simulation.
+  intros. split; [| split].
+  { intros.
+    destruct H0 as [? | [? | ?]]; 
+      inversion H0; subst; inversion H; subst; auto. }
+  { intros.
+    inversion H0; subst; inversion H; subst;
+      constructor; auto. }
+  {
+    intros.
+    inversion H; subst.
+    - exists c1', k1'; split; constructor; auto.
+    - inversion H0; subst.
+      exists (CIf b (CSeq c0 c4) (CSeq c3 c4)), k2;
+      split; [apply rt_refl | constructor].
+    - inversion H0; subst.
+      + exists (CIf b' (CSeq c0 c4) (CSeq c3 c4)), k2; split; constructor.
+        constructor; auto.
+      + exists c1', (KSeq c4 :: k2); split; [| constructor].
+        apply (rt_trans _ _ (CSeq c1' c4, k2, st')); constructor; constructor.
+      + exists c1', (KSeq c4 :: k2); split; [| constructor].
+        apply (rt_trans _ _ (CSeq c1' c4, k2, st')); constructor; constructor.
+  }
+Qed.
 
 Theorem if_seq_valid_continuation : forall P b c1 c2 c3 Q R1 R2,
-  valid_continuation P (CSeq (CIf b c1 c2) c3) Q R1 R2 ->
-  valid_continuation P (CIf b (CSeq c1 c3) (CSeq c2 c3)) Q R1 R2.
+  valid_continuation P (CIf b (CSeq c1 c3) (CSeq c2 c3)) Q R1 R2 ->
+  valid_continuation P (CSeq (CIf b c1 c2) c3) Q R1 R2.
 Proof.
-Admitted.
+  unfold valid_continuation.
+  intros.
+  specialize (H k H0 H1 H2).
+  pose proof (guard_sim (CIf b (CSeq c1 c3) (CSeq c2 c3))
+    (CSeq (CIf b c1 c2) c3) k k P 
+    if_seq_sim if_seq_sim_is_simulation).
+  apply H3; [constructor | auto].
+Qed.
+
+Inductive loop_noc_sim : (com * continuation) -> (com * continuation) -> Prop :=
+  | LN_sim_id : forall c k, loop_noc_sim (c, k) (c, k)
+  | LN_sim_loopnoc : forall c1 c2 k,
+      nocontinue_c c1 -> nocontinue_c c2 ->
+      loop_noc_sim (CFor c1 c2, k) (CFor (CSeq c1 c2) CSkip, k)
+  | LN_sim_1 : forall c1 c2 k,
+      nocontinue_c c1 -> nocontinue_c c2 ->
+      loop_noc_sim (CSeq c1 CCont, KLoop1 c1 c2 :: k) 
+        (CSeq c1 c2, KSeq CCont :: KLoop1 (CSeq c1 c2) CSkip :: k)
+  | LN_sim_2 : forall c0 c1 c2 k k0,
+      nocontinue c0 k0 -> nocontinue_c c1 -> nocontinue_c c2 ->
+      loop_noc_sim (c0, k0 ++ KSeq CCont :: KLoop1 c1 c2 :: k)
+        (c0, k0 ++ KSeq c2 :: KSeq CCont :: KLoop1 (CSeq c1 c2) CSkip :: k)
+  | LN_sim_3 : forall c1 c2 k,
+      nocontinue_c c1 -> nocontinue_c c2 ->
+      loop_noc_sim (CCont, KLoop1 c1 c2 :: k) 
+        (c2, KSeq CCont :: KLoop1 (CSeq c1 c2) CSkip :: k)
+  | LN_sim_4 : forall c0 c1 c2 k k0,
+      nocontinue c0 k0 -> nocontinue_c c1 -> nocontinue_c c2 ->
+      loop_noc_sim (c0, k0 ++ KLoop2 c1 c2 :: k)
+        (c0, k0 ++ KSeq CCont :: KLoop1 (CSeq c1 c2) CSkip :: k)
+  | LN_sim_5 : forall c1 c2 k,
+      nocontinue_c c1 -> nocontinue_c c2 ->
+      loop_noc_sim (CSkip, KLoop2 c1 c2 :: k)
+        (CSkip, KLoop2 (CSeq c1 c2) CSkip :: k)
+  | LN_sim_6 : forall c1 c2 k,
+      nocontinue_c c1 -> nocontinue_c c2 ->
+      loop_noc_sim (CBreak, KLoop1 c1 c2 :: k)
+        (CBreak, KLoop1 (CSeq c1 c2) CSkip :: k).
+
+Lemma loop_noc_sim_is_simulation : simulation loop_noc_sim.
+Proof.
+  unfold simulation.
+  intros.
+  split; [ | split].
+  { intros; destruct H0 as [? | [? | ?]];
+      inversion H0; subst; inversion H; subst;
+      try auto; exfalso; eapply nil_app_neq; rewrite H2; auto. }
+  { intros.
+    inversion H0; subst. inversion H; subst; try tauto.
+    + constructor; auto.
+    + assert (irreducible CSkip
+      (k1 ++ KSeq c5 :: KSeq CCont :: KLoop1 (CSeq c4 c5) CSkip :: k0) st).
+      { destruct k1; inversion H2; subst; constructor. }
+      constructor; auto.
+    + assert (irreducible CSkip 
+      (k1 ++ KSeq CCont :: KLoop1 (CSeq c4 c5) CSkip :: k0) st).
+      { destruct k1; inversion H2; subst; constructor. }
+      constructor; auto.
+    + assert (irreducible c2 k2 st).
+      { inversion H; subst; try tauto.
+        - destruct k1; inversion H2; subst; constructor.
+        - destruct k1; [inversion H5; subst; destruct H1; inversion H1 |
+            inversion H2; subst; constructor]. }
+      constructor; auto. }
+  intros.
+  inversion H; subst. 
+  + exists c1', k1'.
+    split; [ constructor; auto | constructor].
+  + rename c0 into c1; rename c3 into c2; rename k2 into k.
+    inversion H0; subst.
+    exists (CSeq c1 c2), (KSeq CCont :: KLoop1 (CSeq c1 c2) CSkip :: k).
+    split; [ | constructor; auto].
+    eapply rt_trans_1n; [constructor | repeat constructor].
+  + rename c0 into c1; rename c3 into c2.
+    inversion H0; subst c1'; subst.
+    exists c1, (KSeq c2 :: KSeq CCont :: KLoop1 (CSeq c1 c2) CSkip :: k).
+    split; [| apply (LN_sim_2 c1 _ _ _ nil); auto].
+    apply rt_step; constructor.
+    unfold nocontinue; constructor; [left; tauto | constructor].
+  + rename c2 into c0; rename c3 into c1; rename c4 into c2.
+    inversion H0; subst.
+    - exists (CAss X a'), 
+        (k0 ++ KSeq c2 :: KSeq CCont :: KLoop1 (CSeq c1 c2) CSkip :: k).
+      split; [repeat constructor; auto | constructor; auto].
+    - exists CSkip, 
+        (k0 ++ KSeq c2 :: KSeq CCont :: KLoop1 (CSeq c1 c2) CSkip :: k).
+      split; [repeat constructor; auto | constructor; auto].
+    - rename c1' into c01; rename c4 into c02.
+      exists c01,
+        (KSeq c02 :: k0 ++ KSeq c2 :: KSeq CCont :: KLoop1 (CSeq c1 c2) CSkip :: k).
+      split; [repeat constructor; auto |].
+      apply (LN_sim_2 c01 _ _ _ (KSeq c02 :: k0)); auto.
+      unfold nocontinue in *; simpl in *; tauto.
+    - destruct k0.
+      { inversion H3; subst.
+        exists c2, (KSeq CCont :: KLoop1 (CSeq c1 c2) CSkip :: k).
+        split; [repeat constructor; auto | constructor; auto]. }
+      inversion H3; subst. 
+      exists c1',
+        (k1 ++ KSeq c2 :: KSeq CCont :: KLoop1 (CSeq c1 c2) CSkip :: k).
+      split; [repeat constructor; auto | constructor; auto].
+      unfold nocontinue in *; simpl in *; tauto.
+    - destruct k0.
+      { unfold nocontinue in H5; simpl in H5; tauto. }
+      inversion H3; subst.
+      exists CCont, 
+        (k1 ++ KSeq c2 :: KSeq CCont :: KLoop1 (CSeq c1 c2) CSkip :: k).
+      split; [repeat constructor; auto | constructor; auto].
+      unfold nocontinue in *; simpl in *; tauto.
+    - destruct k0.
+      { inversion H3; subst.
+        exists CBreak,
+          (KLoop1 (CSeq c1 c2) CSkip :: k).
+        split; [| constructor; auto].
+        eapply rt_trans_1n; [constructor |].
+        repeat constructor. }
+      inversion H3; subst.
+      exists CBreak,  
+        (k1 ++ KSeq c2 :: KSeq CCont :: KLoop1 (CSeq c1 c2) CSkip :: k).
+      split; [repeat constructor; auto | constructor; auto].
+      unfold nocontinue in *; simpl in *; tauto.
+    - rename c3 into c01; rename c4 into c02.
+      exists (CIf b' c01 c02),
+        (k0 ++ KSeq c2 :: KSeq CCont :: KLoop1 (CSeq c1 c2) CSkip :: k).
+      split; [repeat constructor; auto | constructor; auto].
+    - rename c1' into c01; rename c4 into c02.
+      exists c01,
+        (k0 ++ KSeq c2 :: KSeq CCont :: KLoop1 (CSeq c1 c2) CSkip :: k).
+      split; [repeat constructor; auto | constructor; auto].
+      unfold nocontinue in *; simpl in *; tauto.
+    - rename c3 into c01; rename c1' into c02.
+      exists c02,
+        (k0 ++ KSeq c2 :: KSeq CCont :: KLoop1 (CSeq c1 c2) CSkip :: k).
+      split; [repeat constructor; auto | constructor; auto].
+      unfold nocontinue in *; simpl in *; tauto.
+    - rename c3 into c01; rename c4 into c02.
+      exists (CSeq c01 CCont),
+        (KLoop1 c01 c02 :: k0 ++ KSeq c2 :: KSeq CCont :: KLoop1 (CSeq c1 c2) CSkip :: k).
+      split; [repeat constructor; auto |].
+      apply (LN_sim_2 _ _ _ _ (KLoop1 c01 c02 :: k0)); auto.
+      unfold nocontinue in *; simpl in *; tauto.
+    - destruct k0.
+      { inversion H3; subst. }
+      inversion H3; subst.
+      exists (CSeq c3 CCont),
+        (KLoop1 c3 c4 :: k2 ++ KSeq c2 :: KSeq CCont :: KLoop1 (CSeq c1 c2) CSkip :: k).
+      split; [repeat constructor; auto |].
+      apply (LN_sim_2 _ _ _ _ (KLoop1 c3 c4 :: k2)); auto.
+      unfold nocontinue in *; simpl in *; tauto.
+    - destruct k0; inversion H3; subst.
+      rename c3 into c01; rename c1' into c02.
+      exists c02,
+        (KLoop2 c01 c02 :: k2 ++ KSeq c2 :: KSeq CCont :: KLoop1 (CSeq c1 c2) CSkip :: k).
+        split; [repeat constructor; auto |].
+        apply (LN_sim_2 _ _ _ _ (KLoop2 c01 c02 :: k2)); auto.
+        unfold nocontinue in *; simpl in *; tauto.
+    - destruct k0; inversion H3; subst.
+      rename c3 into c01; rename c4 into c02.
+      exists CSkip,
+        (k1 ++ KSeq c2 :: KSeq CCont :: KLoop1 (CSeq c1 c2) CSkip :: k).
+      split; [repeat constructor; auto |].
+      apply (LN_sim_2 _ _ _ _ k1); auto.
+      unfold nocontinue in *; simpl in *; tauto.
+    - destruct k0; inversion H3; subst.
+      exists CSkip,
+        (k1 ++ KSeq c2 :: KSeq CCont :: KLoop1 (CSeq c1 c2) CSkip :: k).
+      split; [repeat constructor; auto |].
+      apply (LN_sim_2 _ _ _ _ k1); auto.
+      unfold nocontinue in *; simpl in *; tauto.
+    - rename c1' into c00; rename c4 into c01; rename c5 into c02.
+      exists c00,
+        (KLoop1 c01 c02 :: k0 ++ KSeq c2 :: KSeq CCont :: KLoop1 (CSeq c1 c2) CSkip :: k).
+      split; [repeat constructor; auto |].
+      apply (LN_sim_2 _ _ _ _ (KLoop1 c01 c02 :: k0)); auto.
+      unfold nocontinue in *; simpl in *; tauto.
+    - rename c1' into c00; rename c4 into c01; rename c5 into c02.
+      exists c00,
+        (KLoop2 c01 c02 :: k0 ++ KSeq c2 :: KSeq CCont :: KLoop1 (CSeq c1 c2) CSkip :: k).
+      split; [repeat constructor; auto |].
+      apply (LN_sim_2 _ _ _ _ (KLoop2 c01 c02 :: k0)); auto.
+      unfold nocontinue in *; simpl in *; tauto.
+  + inversion H0; subst.
+    rename c0 into c1; rename c1' into c2. 
+    exists c2, (KSeq CCont :: KLoop1 (CSeq c1 c2) CSkip :: k).
+    split;[| apply (LN_sim_4 _ _ _ _ nil); auto].
+    apply rt_refl.
+    unfold nocontinue in *; simpl in *; tauto.
+  + rename c2 into c0; rename c3 into c1; rename c4 into c2.
+    inversion H0; subst.
+    - exists (CAss X a'),
+        (k0 ++ KSeq CCont :: KLoop1 (CSeq c1 c2) CSkip :: k).
+      split; [repeat constructor; tauto | constructor; tauto].
+    - exists CSkip,
+        (k0 ++ KSeq CCont :: KLoop1 (CSeq c1 c2) CSkip :: k).
+      split; [repeat constructor; tauto | constructor; tauto].
+    - rename c1' into c01; rename c4 into c02.
+      exists c01,
+        (KSeq c02 :: k0 ++ KSeq CCont :: KLoop1 (CSeq c1 c2) CSkip :: k).
+      split; [repeat constructor; tauto | ].
+      apply (LN_sim_4 _ _ _ _ (KSeq c02 :: k0)); auto.
+      unfold nocontinue in *; simpl in *; tauto.
+    - destruct k0; inversion H3; subst.
+      exists c1', 
+        (k1 ++ KSeq CCont :: KLoop1 (CSeq c1 c2) CSkip :: k).
+      split; [repeat constructor; auto | constructor; auto].
+      unfold nocontinue in *; simpl in *; tauto.
+    - destruct k0; inversion H3; subst.
+      exists CCont, (k1 ++ KSeq CCont :: KLoop1 (CSeq c1 c2) CSkip :: k).
+      split; [repeat constructor; tauto | constructor; auto].
+      unfold nocontinue in *; simpl in *; tauto.
+    - destruct k0; inversion H3; subst.
+      exists CBreak, (k1 ++ KSeq CCont :: KLoop1 (CSeq c1 c2) CSkip :: k).
+      split; [repeat constructor; auto | constructor; auto].
+      unfold nocontinue in *; simpl in *; tauto.
+    - exists (CIf b' c3 c4),
+        (k0 ++ KSeq CCont :: KLoop1 (CSeq c1 c2) CSkip :: k).
+      split; [repeat constructor; auto | constructor; auto].
+    - exists (c1'),
+        (k0 ++ KSeq CCont :: KLoop1 (CSeq c1 c2) CSkip :: k).
+      split; [repeat constructor; auto | constructor; auto].
+      unfold nocontinue in *; simpl in *; tauto.
+    - exists (c1'),
+        (k0 ++ KSeq CCont :: KLoop1 (CSeq c1 c2) CSkip :: k).
+       split; [repeat constructor; auto | constructor; auto].
+       unfold nocontinue in *; simpl in *; tauto.
+    - rename c3 into c01; rename c4 into c02.
+      exists (CSeq c01 CCont),
+        (KLoop1 c01 c02 :: k0 ++ KSeq CCont :: KLoop1 (CSeq c1 c2) CSkip :: k).
+      split; [repeat constructor; auto |].
+      apply (LN_sim_4 _ _ _ _ (KLoop1 c01 c02 :: k0)); auto.
+      unfold nocontinue in *; simpl in *; tauto.
+    - destruct k0.
+      { inversion H3; subst; simpl in *.
+        exists (CSeq c1 c2),
+          (KSeq CCont :: KLoop1 (CSeq c1 c2) CSkip :: k).
+        split; [| constructor; auto].
+        eapply rt_trans_1n; [constructor |].
+        eapply rt_trans_1n; [constructor |].
+        eapply rt_trans_1n; [constructor |].
+        repeat constructor. }
+      rename c3 into c01; rename c4 into c02.
+      inversion H3; subst.
+      exists (CSeq c01 CCont),
+        (KLoop1 c01 c02 :: k2 ++ KSeq CCont :: KLoop1 (CSeq c1 c2) CSkip :: k).
+      split; [repeat constructor; auto |].
+      apply (LN_sim_4 _ _ _ _ (KLoop1 c01 c02 :: k2)); auto.
+      unfold nocontinue in *; simpl in *; tauto.
+    - destruct k0.
+      { inversion H3; subst. }
+      rename c3 into c01; rename c1' into c02.
+      inversion H3; subst.
+      exists c02,
+        (KLoop2 c01 c02 :: k2 ++ KSeq CCont :: KLoop1 (CSeq c1 c2) CSkip :: k).
+      split; [repeat constructor; auto |].
+      apply (LN_sim_4 _ _ _ _ (KLoop2 c01 c02 :: k2)); auto.
+      unfold nocontinue in *; simpl in *; tauto.
+    - destruct k0.
+      { inversion H3; subst. }
+      rename c3 into c01; rename c4 into c02.
+      inversion H3; subst.
+      exists CSkip,
+        (k1 ++ KSeq CCont :: KLoop1 (CSeq c1 c2) CSkip :: k).
+      split; [repeat constructor; auto |].
+      apply (LN_sim_4 _ _ _ _ k1); auto.
+      unfold nocontinue in *; simpl in *; tauto.
+    - destruct k0.
+      { inversion H3; subst.
+        simpl in *.
+        exists CSkip, k; split; [| constructor].
+        eapply rt_trans_1n; [constructor |].
+        eapply rt_trans_1n; [constructor |].
+        apply rt_refl. }
+      rename c3 into c01; rename c4 into c02.
+      inversion H3; subst.
+      exists CSkip,
+        (k1 ++ KSeq CCont :: KLoop1 (CSeq c1 c2) CSkip :: k).
+      split; [repeat constructor; auto |].
+      apply (LN_sim_4 _ _ _ _ k1); auto.
+      unfold nocontinue in *; simpl in *; tauto.
+      - rename c1' into c00; rename c4 into c01; rename c5 into c02.
+      exists c00,
+        (KLoop1 c01 c02 :: k0 ++ KSeq CCont :: KLoop1 (CSeq c1 c2) CSkip :: k).
+      split; [repeat constructor; auto |].
+      apply (LN_sim_4 _ _ _ _ (KLoop1 c01 c02 :: k0)); auto.
+      unfold nocontinue in *; simpl in *; tauto.
+    - rename c1' into c00; rename c4 into c01; rename c5 into c02.
+      exists c00,
+        (KLoop2 c01 c02 :: k0 ++ KSeq CCont :: KLoop1 (CSeq c1 c2) CSkip :: k).
+      split; [repeat constructor; auto |].
+      apply (LN_sim_4 _ _ _ _ (KLoop2 c01 c02 :: k0)); auto.
+      unfold nocontinue in *; simpl in *; tauto.
+  + rename c0 into c1; rename c3 into c2.
+    inversion H0; subst.
+    exists (CSeq c1 c2),
+      (KSeq CCont :: KLoop1 (CSeq c1 c2) CSkip :: k).
+    split; [| constructor; auto].
+    eapply rt_trans_1n; [constructor; auto|].
+    eapply rt_trans_1n; [constructor; auto|].
+    apply rt_refl.
+  + inversion H0; subst.
+    rename c0 into c1; rename c3 into c2.
+    exists CSkip, k1'.
+    split; [repeat constructor | constructor].
+Qed.
 
 Theorem loop_nocontinue_valid_continuation : forall P c1 c2 Q R1 R2,
-  nocontinue c1 ->
-  nocontinue c2 ->
+  nocontinue_c c1 ->
+  nocontinue_c c2 ->
   valid_continuation P (CFor (CSeq c1 c2) CSkip) Q R1 R2 ->
   valid_continuation P (CFor c1 c2) Q R1 R2.
 Proof.
   unfold valid_continuation.
   intros.
-Admitted. 
+  specialize (H1 k H2 H3 H4).
+  pose proof (guard_sim (CFor (CSeq c1 c2) CSkip)
+    (CFor c1 c2) k k P 
+    loop_noc_sim loop_noc_sim_is_simulation).
+  apply H5; try tauto; constructor; auto.
+Qed.
